coq/theories/imp2asm/ImpToASMCodegenProofs.v
@@ -67,27 +67,47 @@ Definition has_stack (t : ASMSemantics.state) (xs : list word_or_ret) : Prop :=
     t.(regs) RAX = Some w /\
     t.(stack) = ws.
 
+Definition v_arr_inv (asmm: word64 -> option (option word64))
+  (block: list (option Value)) (vasm: option word64): Prop :=
+  forall i v,
+    List.nth_error block i = Some v ->
+    exists w,
+      v = Some (ImpSyntax.Word w) /\
+      match vasm with
+      | Some base =>
+          asmm (word.add base (word.of_Z (Z.of_nat i * 8))) = Some (Some w)
+      | None => False
+      end.
+
 (* Constrains v to valid ranges and equates it with w in the context of ASM state t. *)
-Definition v_inv (t : ASMSemantics.state) (v : Value) (w : word64) : Prop :=
+Definition v_inv (asmm: word64 -> option (option word64)) (impm: list (list (option Value)))
+  (v: Value) (w: word64): Prop :=
   match v with
   | ImpSyntax.Word v => word.ltu v (word.of_Z (2 ^ 63)) = true /\ w = v
-  | Pointer v => t.(memory) w <> None (* TODO(kπ) assert equality of memory blocks? *)
+  | Pointer p =>
+    match List.nth_error impm p, asmm w with
+    | Some block, Some asmv =>
+      v_arr_inv asmm block asmv
+    | _, _ => False
+    end
   end.
 
 (* Checks that environment variables map to valid locations and values on the stack in the ASM state. *)
-Definition env_ok (env : IEnv.env) (vs : list (option nat)) (curr : list word_or_ret) (t : ASMSemantics.state) : Prop :=
+Definition env_ok (env : IEnv.env) (vs : list (option nat)) (curr : list word_or_ret)
+  (asmm : word64 -> option (option word64))
+  (impm: list (list (option Value))): Prop :=
   List.length vs = List.length curr /\
   forall n v,
     IEnv.lookup env n = Some v ->
     index_of n 0 vs < List.length curr /\
     exists w,
       nth_error curr (index_of n 0 vs) = Some (Word w) /\
-      v_inv t v w.
+      v_inv asmm impm v w.
 
 Definition cmd_res_rel (ri: outcome Value unit) (l1: nat) (stck: list word_or_ret) (t1: ASMSemantics.state) (s1: ImpSemantics.state) : Prop :=
   match ri with
   | Stop (Return v) => exists w,
-    v_inv t1 v w /\
+    v_inv t1.(memory) s1.(ImpSemantics.memory) v w /\
     has_stack t1 (Word w :: stck) /\
     t1.(pc) = l1
   | Cont _ =>
@@ -99,7 +119,7 @@ Definition cmd_res_rel (ri: outcome Value unit) (l1: nat) (stck: list word_or_re
 Definition exp_res_rel (ri: outcome Value Value) (l1: nat) (stck: list word_or_ret) (t1: ASMSemantics.state) (s1: ImpSemantics.state) : Prop :=
   match ri with
   | Cont v => exists w,
-    v_inv t1 v w /\
+    v_inv t1.(memory) s1.(ImpSemantics.memory) v w /\
     has_stack t1 (Word w :: stck) /\
     t1.(pc) = l1
   | _ => False
@@ -117,7 +137,7 @@ Definition goal_exp (e : exp): Prop :=
     res <> Stop Crash ->
     c_exp e t.(pc) vs = (asmc, l1) ->
     state_rel fs s t ->
-    env_ok s.(vars) vs curr t ->
+    env_ok s.(vars) vs curr t.(memory) s.(ImpSemantics.memory) ->
     has_stack t (curr ++ rest) ->
     odd (List.length rest) = true ->
     code_in t.(pc) (flatten asmc) t.(instructions) ->
@@ -143,7 +163,7 @@ Definition goal_cmd (c : cmd): Prop :=
     res <> Stop Crash ->
     c_cmd c t.(pc) fs vs = (asmc, l1, vs') ->
     state_rel fs s t ->
-    env_ok s.(vars) vs curr t ->
+    env_ok s.(vars) vs curr t.(memory) s.(ImpSemantics.memory) ->
     has_stack t (curr ++ rest) ->
     odd (List.length rest) = true ->
     code_in t.(pc) (flatten asmc) t.(instructions) ->
@@ -328,6 +348,36 @@ Theorem substring_noop: forall s,
 Proof.
 Admitted.
 
+Ltac bound_crunch :=
+  intros;
+  try rewrite word.unsigned_ltu in *;
+  try rewrite word.unsigned_of_Z in *;
+  try unfold word.wrap in *;
+  (* THIS IS HORRIBLY SLOW *)
+  cbn in *;
+  lia.
+
+Theorem sub_lt_bound: forall (a b: Z),
+  (a <? b)%Z = true ->
+  (a <? Z.pow_pos 2 63 mod Z.pow_pos 2 64)%Z = true ->
+  (b <? Z.pow_pos 2 63 mod Z.pow_pos 2 64)%Z = true ->
+  ((b - a) mod Z.pow_pos 2 64 <? Z.pow_pos 2 63 mod Z.pow_pos 2 64)%Z = true.
+Proof.
+Admitted.
+
+Theorem z_lt_bound: forall (z: Z),
+  word.ltu (word.of_Z (2 ^ 63 - 1)) ((Naive.wrap z): word64) = false ->
+  (z mod Z.pow_pos 2 64 <? Z.pow_pos 2 63 mod Z.pow_pos 2 64)%Z = true.
+Proof.
+  intros.
+  rewrite word.unsigned_ltu in *.
+  rewrite word.unsigned_of_Z in *.
+  unfold word.wrap in *.
+  (* THIS IS HORRIBLY SLOW *)
+  cbn in *.
+  lia.
+Qed.
+
 Theorem w_lt_bound: forall (w: word64),
   (word.ltu (word.of_Z (2 ^ 63 - 1)) w = false \/
     word.ltu w (word.of_Z (2 ^ 63)) = true) ->
@@ -342,6 +392,174 @@ Proof.
   cbn in *.
   lia.
 Qed.
+
+Theorem c_exp_length: forall e l vs c l1,
+  c_exp e l vs = (c, l1) -> l1 = l + List.length (flatten c).
+Proof.
+  induction e.
+  all: intros.
+  all: simpl c_exp in *.
+  all: repeat match goal with
+  | [ H : context[(if ?x then _ else _)] |- _ ] => destruct x eqn:?
+  | [ H : context [(match ?x with | _ => _ end)] |- _ ] => destruct x eqn:?
+  | [ H : (_, _) = (_, _) |- _ ] => inversion H; subst; clear H
+  | [ |- context[ fst ?x ] ] => destruct x eqn:?; simpl in *
+  | [ H : c_exp _ _ (None :: _) = (_, _) |- _ ] => eapply IHe2 in H; subst
+  | [ H : c_exp _ _ ?_l = (_, _) |- _ ] => eapply IHe1 in H; subst
+  | _ => progress unfold c_var, c_const, dlet in *
+  | _ => progress simpl in *
+  | _ => progress rewrite length_app
+  | _ => lia
+  end.
+Qed.
+
+Theorem code_in_append: forall xs ys n code,
+    code_in n (xs ++ ys) code <->
+    (code_in n xs code ∧ code_in (n + List.length xs) ys code).
+Proof.
+  induction xs; intros; simpl.
+  - split; intros; cleanup; try split; eauto.
+    all: rewrite Nat.add_0_r in *; eauto.
+  - split; intros; cleanup.
+    + repeat split; eauto.
+      all: eapply IHxs in H0; cleanup; eauto.
+      rewrite <- Nat.add_1_l.
+      rewrite Nat.add_assoc.
+      eauto.
+    + repeat split; eauto.
+      all: eapply IHxs; cleanup; eauto.
+      repeat split; eauto.
+      rewrite <- Nat.add_1_l in H0.
+      rewrite Nat.add_assoc in H0.
+      eauto.
+Qed.
+
+Theorem eval_exp_not_stop: forall e s res s1 v,
+  eval_exp e s = (res, s1) ->
+  res ≠ Stop Crash ->
+  res <> Stop v.
+Proof.
+  induction e; intros.
+  all: simpl eval_exp in *.
+  all: unfold lookup_var, bind in *; unfold_outcome; simpl in *.
+  - destruct (IEnv.lookup (vars s) n) eqn:?.
+    all: inversion H; subst; congruence.
+  - congruence.
+  - destruct (eval_exp e1 s) eqn:?; destruct o eqn:?.
+    2: unfold not; intros; inversion H; subst; eapply IHe1 in Heqp; inversion H3; subst; eauto.
+    destruct (eval_exp e2 s0) eqn:?; destruct o0 eqn:?.
+    2: unfold not; intros; inversion H; subst; eapply IHe2 in Heqp0; inversion H3; subst; eauto.
+    unfold combine_word in *.
+    destruct v0; unfold_outcome.
+    2: congruence.
+    destruct v1; unfold_outcome.
+    all: congruence.
+  - destruct (eval_exp e1 s) eqn:?; destruct o eqn:?.
+    2: unfold not; intros; inversion H; subst; eapply IHe1 in Heqp; inversion H3; subst; eauto.
+    destruct (eval_exp e2 s0) eqn:?; destruct o0 eqn:?.
+    2: unfold not; intros; inversion H; subst; eapply IHe2 in Heqp0; inversion H3; subst; eauto.
+    unfold combine_word in *.
+    destruct v0; unfold_outcome.
+    2: congruence.
+    destruct v1; unfold_outcome.
+    all: congruence.
+  - destruct (eval_exp e1 s) eqn:?; destruct o eqn:?.
+    2: unfold not; intros; inversion H; subst; eapply IHe1 in Heqp; inversion H3; subst; eauto.
+    destruct (eval_exp e2 s0) eqn:?; destruct o0 eqn:?.
+    2: unfold not; intros; inversion H; subst; eapply IHe2 in Heqp0; inversion H3; subst; eauto.
+    destruct (value_eqb v1 (ImpSyntax.Word (Naive.wrap 0))) eqn:?.
+    1: congruence.
+    unfold combine_word in *.
+    destruct v0; unfold_outcome.
+    2: congruence.
+    destruct v1; unfold_outcome.
+    all: congruence.
+  - destruct (eval_exp e1 s) eqn:?; destruct o eqn:?.
+    2: unfold not; intros; inversion H; subst; eapply IHe1 in Heqp; inversion H3; subst; eauto.
+    destruct (eval_exp e2 s0) eqn:?; destruct o0 eqn:?.
+    2: unfold not; intros; inversion H; subst; eapply IHe2 in Heqp0; inversion H3; subst; eauto.
+    unfold mem_load in *.
+    destruct v0; unfold_outcome.
+    1: congruence.
+    destruct v1; unfold_outcome.
+    2: congruence.
+    destruct (negb (w2n w mod 8 =? 0)) eqn:?.
+    1: congruence.
+    destruct (nth_error (ImpSemantics.memory s2) i) eqn:?.
+    2: congruence.
+    destruct (nth_error _ (w2n w / 8)) eqn:?.
+    2: congruence.
+    destruct o1 eqn:?.
+    all: congruence.
+Qed.
+
+Theorem steps_instructions: forall s1 s2 f1 f2,
+  steps (State s1, f1) (State s2, f2) -> s1.(instructions) = s2.(instructions).
+Proof.
+Admitted.
+
+Theorem index_of_spec: forall name vs k,
+  index_of name k vs = k + index_of name 0 vs.
+Proof.
+  induction vs; intros; eauto.
+  simpl; destruct a.
+  - destruct (_ =? _) eqn:?; simpl; eauto.
+    rewrite IHvs; eapply eq_sym; rewrite IHvs.
+    rewrite Nat.add_assoc.
+    reflexivity.
+  - rewrite IHvs; eapply eq_sym; rewrite IHvs.
+    rewrite Nat.add_assoc.
+    reflexivity.
+Qed.
+
+Ltac crunch_give_up_even :=
+  repeat match  goal with
+  | |- (ImpToASMCodegen.give_up _) = (ImpToASMCodegen.give_up _) => f_equal
+  | |- context[even_len _] => rewrite even_len_spec
+  | |- context[odd_len _] => rewrite odd_len_spec
+  | [ H: (List.length ?vs = _) |- context[List.length ?vs] ] => rewrite H
+  | |- context[List.length (_ ++ _)] => rewrite length_app
+  | |- context[odd (_ + _)] => rewrite Nat.odd_add
+  | |- context[even (_ + _)] => rewrite Nat.even_add
+  | [ H: odd ?x = _ |- context[odd ?x] ] => rewrite H
+  | [ H: (even (List.length (stack ?t))) = _ |- context C [odd (List.length (stack ?t))]] =>
+    repeat rewrite <- Nat.negb_even; rewrite H; clear H
+  | [ H: (odd (List.length (stack ?t))) = _ |- context C [even (List.length (stack ?t))]] =>
+    repeat rewrite <- Nat.negb_even; rewrite H; clear H
+  | [ H: (even (List.length (stack ?t))) = _ |- context C [even (List.length (stack ?t))]] =>
+    rewrite H; clear H
+  | [ H: (odd (List.length (stack ?t))) = _ |- context C [odd (List.length (stack ?t))]] =>
+    rewrite H; clear H
+  | _ => rewrite xorb_true_r || rewrite Nat.negb_odd || rewrite Nat.negb_even
+  | _ => tauto
+end.
+
+Theorem env_ok_add_None: forall vars vs curr x asmm impm,
+  env_ok vars vs curr asmm impm ->
+  env_ok vars (None :: vs) (Word x :: curr) asmm impm.
+Proof.
+  intros * H.
+  unfold env_ok in *; cleanup.
+  split.
+  1: simpl; eauto.
+  intros*; intro HLookup.
+  eapply H0 in HLookup; cleanup.
+  split; try eexists; try split.
+  all: simpl.
+  all: try rewrite index_of_spec; try lia.
+  all: unfold v_inv in *.
+  1: simpl; eapply H2.
+  destruct v; [assumption|].
+  assumption.
+Qed.
+
+Ltac rw tac :=
+  let n := fresh "H" in
+  ltac:(tac); intros n; rewrite n in *; clear n.
+
+Ltac rwr tac :=
+  let n := fresh "H" in
+  ltac:(tac); intros n; rewrite <- n in *; clear n.
 
 Theorem c_exp_Const : forall (w: word64),
   goal_exp (ImpSyntax.Const w).
@@ -370,21 +588,8 @@ Proof.
         all: unfold state_rel in *; cleanup.
         eapply give_up.
         all: unfold_stack; eauto.
-        rewrite odd_len_spec.
-        unfold env_ok in *.
-        cleanup.
-        rewrite H3 in *.
-        f_equal.
-        apply eq_sym.
-        rewrite <- Nat.negb_even.
-        rewrite H7.
-        rewrite Nat.negb_odd.
-        rewrite length_app.
-        rewrite Nat.even_add.
-        repeat rewrite <- Nat.negb_odd.
-        rewrite H5.
-        rewrite Nat.negb_odd.
-        tauto.
+        unfold env_ok in *; cleanup.
+        crunch_give_up_even.
     - simpl.
       split; try reflexivity.
       inversion H; subst.
@@ -393,7 +598,6 @@ Proof.
       rewrite prefix_correct.
       apply substring_noop.
   }
-  simpl.
   inversion H1; subst; clear H1.
   simpl flatten in *.
   eexists.
@@ -401,12 +605,10 @@ Proof.
   1: {
     eapply steps_trans.
     + eapply steps_step_same.
-      simpl code_in in *.
-      cleanup.
+      simpl code_in in *; cleanup.
       eapply step_push in e; eauto.
     + eapply steps_step_same.
-      simpl code_in in *.
-      cleanup.
+      simpl code_in in *; cleanup.
       eapply step_const with (w := w).
       eauto.
   }
@@ -561,17 +763,292 @@ Theorem c_exp_Add : forall (e1 e2: exp),
   goal_exp (ImpSyntax.Add e1 e2).
 Proof.
   intros.
-  unfold goal_exp.
-  intros.
-  unfold has_stack in *; cleanup.
+  unfold goal_exp; intros.
   simpl eval_exp in *.
-
-  unfold lookup_var in *.
-  unfold state_rel in *; cleanup.
-  unfold env_ok in *; cleanup.
-  unfold code_rel in *; cleanup.
   simpl c_exp in *; unfold c_add in *; unfold dlet in *.
-  (* unfold goal_exp in H. *)
-  (* specialize H with (t := t) (vs := vs) (s := s) (s1 := s1) (fuel := fuel). *)
+  destruct (eval_exp e1 s) eqn:?; simpl in *; unfold bind at 1 in H1; rewrite Heqp in *; subst.
+  destruct o eqn:?; subst.
+  2: {
+    destruct v eqn:?; subst.
+    all: inversion H1; subst.
+    all: eapply eval_exp_not_stop in Heqp; unfold not in *; eauto; exfalso; apply Heqp; eauto.
+  }
+  destruct (eval_exp e2 s0) eqn:?; simpl in *; unfold bind at 1 in H1; rewrite Heqp0 in H1; subst.
+  destruct o eqn:?; subst.
+  2: {
+    destruct v eqn:?; subst.
+    all: inversion H1; subst.
+    all: eapply eval_exp_not_stop in Heqp0; unfold not in *; eauto; exfalso; apply Heqp0; eauto.
+  }
+  unfold combine_word in *.
+  destruct v eqn:?.
+  2: inversion H1; subst; contradiction.
+  destruct v0 eqn:?.
+  2: inversion H1; subst; contradiction.
+  unfold_outcome; inversion H1; subst.
   destruct (c_exp e1 (pc t) vs) eqn:?; simpl in *.
+  destruct (c_exp e2 n (None :: vs)) eqn:?; simpl in *.
+  specialize (eval_exp_pure e1 _ _ _ Heqp).
+  specialize (eval_exp_pure e2 _ _ _ Heqp0).
+  intros; subst.
+  unfold goal_exp in H; eapply H in Heqp; clear H; eauto; inversion H3; subst.
+  all: simpl flatten in *.
+  all: repeat rewrite code_in_append in *; cleanup.
+  all: try congruence.
+  rwr ltac:(specialize (c_exp_length e1 _ _ _ _ Heqp1)).
+  specialize (c_exp_length e2 _ _ _ _ Heqp2) as ?; subst.
+  destruct x; destruct s; cleanup.
+  2: eexists; split; eauto; simpl; split; eauto.
+  unfold exp_res_rel in *; cleanup.
+  unfold goal_exp in H0.
+  rewrite <- H15 in *.
+  rw ltac:(specialize (steps_instructions _ _ _ _ H10)).
+  eapply H0 in Heqp0; clear H0; eauto; inversion H3; clear H3; subst; cleanup; eauto.
+  2: congruence.
+  1: destruct x0; destruct s0; cleanup; subst.
+  2: eexists; split; [eapply steps_trans|]; eauto; simpl; split; eauto.
+  all: unfold exp_res_rel in *; cleanup.
+  1: instantiate (1 := (Word x :: curr)) in H15; simpl in *; cleanup.
+  1: {
+    unfold state_rel in *; cleanup.
+    specialize (has_stack_even t (curr ++ rest) H6) as ?.
+    specialize (has_stack_even _ _ H14) as ?.
+    specialize (has_stack_even _ _ H15) as ?.
+    unfold has_stack in *; cleanup; subst.
+    unfold env_ok in *; cleanup.
+    inversion H15; clear H15; subst.
+    inversion H14; clear H14; subst.
+    rw ltac:(specialize (steps_instructions _ _ _ _ H0)).
+    destruct (word.ltu ((word.of_Z (2 ^ 63 - 1)): word64)
+      (Naive.wrap ((Naive.unsigned x7) + (Naive.unsigned x9)))) eqn:?.
+    1: {
+      eexists.
+      split.
+      1: {
+        eapply steps_trans.
+        1: eapply H10.
+        eapply steps_trans.
+        1: eapply H0.
+        rewrite <- H16 in *.
+        unfold code_in in H9; cleanup; subst.
+        eapply steps_trans.
+        1: eapply steps_step_same.
+        1: eapply step_pop; eauto.
+        eapply steps_trans.
+        1: eapply steps_step_same.
+        1: eapply step_add; eauto.
+        1: unfold_stack; eauto.
+        eapply steps_trans.
+        1: eapply steps_step_same.
+        1: eapply step_jump; eauto.
+        1: unfold_stack; constructor; eauto.
+        1: simpl; eauto.
+        simpl Z.pow in *; unfold Z.pow_pos in *; simpl PosDef.Pos.iter in *; simpl Z.sub in *.
+        rewrite Heqb.
+        unfold_stack.
+        eapply give_up; unfold_stack; eauto.
+        crunch_give_up_even.
+      }
+      simpl.
+      repeat split; eauto.
+      rewrite H21.
+      rewrite prefix_correct.
+      apply substring_noop.
+    }
+    eexists.
+    split.
+    1: {
+      eapply steps_trans.
+      1: eapply H10.
+      eapply steps_trans.
+      1: eapply H0.
+      rewrite <- H16 in *.
+      unfold code_in in H9; cleanup; subst.
+      eapply steps_trans.
+      1: eapply steps_step_same.
+      1: eapply step_pop; [eapply H9|]; eauto.
+      eapply steps_trans.
+      1: eapply steps_step_same.
+      1: eapply step_add; eauto.
+      1: unfold_stack; eauto.
+      eapply steps_trans.
+      1: eapply steps_step_same.
+      1: eapply step_jump; eauto.
+      1: unfold_stack; constructor; eauto.
+      1: simpl; eauto.
+      simpl Z.pow in *; unfold Z.pow_pos in *; simpl PosDef.Pos.iter in *; simpl Z.sub in *.
+      rewrite Heqb.
+      eapply steps_refl.
+    }
+    simpl.
+    repeat split; eauto.
+    all: unfold code_rel in *; cleanup; eauto.
+    1: eexists; eexists; eauto.
+    eexists; repeat split; repeat eexists; eauto.
+    3: rewrite H16; lia.
+    2: rewrite Z.add_comm; reflexivity.
+    unfold v_inv in *; cleanup; subst.
+    eapply z_lt_bound.
+    rewrite Z.add_comm; assumption.
+  }
+  all: eauto.
+  unfold state_rel in *; cleanup.
+  eapply env_ok_add_None; eauto.
+  admit.
 Admitted.
+
+Theorem c_exp_Sub : forall (e1 e2: exp),
+  goal_exp e1 -> goal_exp e2 ->
+  goal_exp (ImpSyntax.Sub e1 e2).
+Proof.
+  intros.
+  unfold goal_exp; intros.
+  simpl eval_exp in *.
+  simpl c_exp in *; unfold c_sub in *; unfold dlet in *.
+  destruct (eval_exp e1 s) eqn:?; simpl in *; unfold bind at 1 in H1; rewrite Heqp in *; subst.
+  destruct o eqn:?; subst.
+  2: {
+    destruct v eqn:?; subst.
+    all: inversion H1; subst.
+    all: eapply eval_exp_not_stop in Heqp; unfold not in *; eauto; exfalso; apply Heqp; eauto.
+  }
+  destruct (eval_exp e2 s0) eqn:?; simpl in *; unfold bind at 1 in H1; rewrite Heqp0 in H1; subst.
+  destruct o eqn:?; subst.
+  2: {
+    destruct v eqn:?; subst.
+    all: inversion H1; subst.
+    all: eapply eval_exp_not_stop in Heqp0; unfold not in *; eauto; exfalso; apply Heqp0; eauto.
+  }
+  unfold combine_word in *.
+  destruct v eqn:?.
+  2: inversion H1; subst; contradiction.
+  destruct v0 eqn:?.
+  2: inversion H1; subst; contradiction.
+  unfold_outcome; inversion H1; subst.
+  destruct (c_exp e1 (pc t) vs) eqn:?; simpl in *.
+  destruct (c_exp e2 n (None :: vs)) eqn:?; simpl in *.
+  specialize (eval_exp_pure e1 _ _ _ Heqp).
+  specialize (eval_exp_pure e2 _ _ _ Heqp0).
+  intros; subst.
+  unfold goal_exp in H; eapply H in Heqp; clear H; eauto; inversion H3; subst.
+  all: simpl flatten in *.
+  all: repeat rewrite code_in_append in *; cleanup.
+  all: try congruence.
+  rwr ltac:(specialize (c_exp_length e1 _ _ _ _ Heqp1)).
+  specialize (c_exp_length e2 _ _ _ _ Heqp2) as ?; subst.
+  destruct x; destruct s; cleanup.
+  2: eexists; split; eauto; simpl; split; eauto.
+  unfold exp_res_rel in *; cleanup.
+  unfold goal_exp in H0.
+  rewrite <- H15 in *.
+  rw ltac:(specialize (steps_instructions _ _ _ _ H10)).
+  eapply H0 in Heqp0; clear H0; eauto; inversion H3; clear H3; subst; cleanup; eauto.
+  2: congruence.
+  1: destruct x0; destruct s0; cleanup; subst.
+  2: eexists; split; [eapply steps_trans|]; eauto; simpl; split; eauto.
+  all: unfold exp_res_rel in *; cleanup.
+  1: instantiate (1 := (Word x :: curr)) in H15; simpl in *; cleanup.
+  1: {
+    unfold state_rel in *; cleanup.
+    specialize (has_stack_even t (curr ++ rest) H6) as ?.
+    specialize (has_stack_even _ _ H14) as ?.
+    specialize (has_stack_even _ _ H15) as ?.
+    unfold has_stack in *; cleanup; subst.
+    unfold env_ok in *; cleanup.
+    inversion H15; clear H15; subst.
+    inversion H14; clear H14; subst.
+    rw ltac:(specialize (steps_instructions _ _ _ _ H0)).
+    destruct (word.ltu x7 x9) eqn:?.
+    1: {
+      eexists.
+      split.
+      1: {
+        eapply steps_trans.
+        1: eapply H10.
+        eapply steps_trans.
+        1: eapply H0.
+        rewrite <- H16 in *.
+        unfold code_in in H9; cleanup; subst.
+        eapply steps_trans.
+        1: eapply steps_step_same.
+        1: eapply step_pop; eauto.
+        eapply steps_trans.
+        1: eapply steps_step_same.
+        1: eapply step_jump; eauto.
+        1: constructor; simpl; eauto.
+        rewrite Heqb.
+        eapply steps_trans.
+        1: eapply steps_step_same.
+        1: eapply step_sub; eauto.
+        1: assert (pc s0 + 3 = pc s0 + 1 + 1 + 1) as -> by lia.
+        1: unfold_stack; eauto.
+        1-2: simpl; eauto.
+        eapply steps_trans.
+        1: eapply steps_step_same.
+        1: eapply step_mov; eauto.
+        1: assert (pc s0 + 3 = pc s0 + 1 + 1 + 1) as -> by lia.
+        1: unfold_stack; eauto.
+        1: simpl; eauto.
+        eapply steps_refl.
+      }
+      simpl.
+      repeat split; eauto.
+      all: unfold code_rel in *; cleanup; eauto.
+      1: eexists; eexists; eauto.
+      eexists; repeat split; repeat eexists; eauto.
+      2: lia.
+      rewrite word.unsigned_ltu in *.
+      eapply sub_lt_bound; eauto.
+    }
+    eexists.
+    split.
+    1: {
+      eapply steps_trans.
+      1: eapply H10.
+      eapply steps_trans.
+      1: eapply H0.
+      rewrite <- H16 in *.
+      unfold code_in in H9; cleanup; subst.
+      eapply steps_trans.
+      1: eapply steps_step_same.
+      1: eapply step_pop; eauto.
+      eapply steps_trans.
+      1: eapply steps_step_same.
+      1: eapply step_jump; eauto.
+      1: constructor; simpl; eauto.
+      rewrite Heqb.
+      eapply steps_trans.
+      1: eapply steps_step_same.
+      1: eapply step_mov; eauto.
+      1: simpl; eauto.
+      eapply steps_trans.
+      1: eapply steps_step_same.
+      1: eapply step_sub; eauto.
+      1: unfold_stack; eauto.
+      1: simpl; eauto.
+      eapply steps_trans.
+      1: eapply steps_step_same.
+      1: eapply step_mov; eauto.
+      1: simpl; eauto.
+      eapply steps_refl.
+    }
+    simpl.
+    repeat split; eauto.
+    all: unfold code_rel in *; cleanup; eauto.
+    1: eexists; eexists; eauto.
+    eexists; repeat split; repeat eexists; eauto.
+    3: lia.
+    1: admit. (* ((Naive.unsigned x9 - Naive.unsigned x7) mod Z.pow_pos 2 64 <?
+Z.pow_pos 2 63 mod Z.pow_pos 2 64)%Z = true *)
+    admit. (* Some (Naive.wrap (Naive.unsigned x9 - Naive.unsigned x9)) =
+Some (Naive.wrap (Naive.unsigned x9 - Naive.unsigned x7)) *)
+  }
+  all: eauto.
+  unfold state_rel in *; cleanup.
+  eapply env_ok_add_None; eauto.
+  admit.
+Admitted.
+
+
+
+
